verified/smcapi.i.dfy
@@ -561,3 +561,83 @@ lemma smchandlerPreservesPageDbValidity(pageDbIn: PageDb, callno: word, arg1: wo
         stopPreservesPageDbValidity(pageDbIn, arg1);
     }
 }
+
+lemma lemma_updateL2PtePreservesPageDb(d:PageDb,a:PageNr,mapping:Mapping,l2e:L2PTE) 
+    requires validPageDb(d)
+    requires isAddrspace(d, a)
+    requires validMapping(mapping,d,a)
+    requires d[a].entry.state.InitState?
+    requires validL2PTE(d,a,l2e)
+    ensures validPageDb(updateL2Pte(d,a,mapping,l2e))
+{
+    reveal_validPageDb();
+    var d' := updateL2Pte(d,a,mapping,l2e);
+    
+    var addrspace := d[a].entry;
+    assert validAddrspace(d, a);
+
+    var l2index := mapping.l2index;
+    var l1index := mapping.l1index;
+
+    var l1p := d[a].entry.l1ptnr;
+    var l1 := d[l1p].entry;
+    var l1p' := d'[a].entry.l1ptnr;
+    var l1' := d'[l1p'].entry;
+    assert l1p' == l1p;
+    assert l1' == l1;
+
+    var l1pte := fromJust(l1.l1pt[l1index]);
+    var l1pte' := fromJust(l1'.l1pt[l1index]);
+    assert l1pte == l1pte';
+    var l2pt := d[l1pte].entry.l2pt;
+    var l2pt' := d'[l1pte].entry.l2pt;
+
+    //it's now okay to drop the primes from everything but l2pt'
+
+    assert !stoppedAddrspace(d[a]);
+    assert !stoppedAddrspace(d'[a]);
+
+    assert validPageDbEntry(d, a);
+    assert validPageDbEntry(d', a) by
+    {
+        assert d'[a].entry.refcount == d[a].entry.refcount;
+        assert addrspaceRefs(d', a) == addrspaceRefs(d, a);
+        
+    }
+
+    assert validPageDbEntry(d, l1p);
+    assert validPageDbEntry(d, l1pte);
+
+    assert validPageDbEntry(d', l1p);
+    assert validPageDbEntry(d', l1pte) by
+    {
+       assert d'[l1pte].entry.L2PTable?;
+       assert !stoppedAddrspace(d'[a]);
+       assert validL2PTE(d',a,l2e);
+       assert wellFormedPageDbEntryTyped(d[l1pte].entry);
+       assert wellFormedPageDbEntryTyped(d'[l1pte].entry);
+
+       assert |l2pt| == |l2pt'|;
+
+       forall ( i | 0 <= i < NR_L2PTES() && i != l2index )
+            ensures validL2PTE(d',a,l2pt'[i])
+       {
+            assert l2pt'[i] == l2pt[i];
+            assert validL2PTE(d,a,l2pt[i]);
+       }
+
+    }
+
+    forall ( p | validPageNr(p) && p != l1p && p != l1pte && p != a )
+        ensures validPageDbEntry(d', p)
+    {
+            assert d'[p] == d[p];
+            assert validPageDbEntry(d, p);
+            assert addrspaceRefs(d', p) == addrspaceRefs(d, p);
+    }
+    
+    assert wellFormedPageDb(d');
+    assert pageDbEntriesValid(d');
+    assert pageDbEntriesValidRefs(d');
+  
+}
